Example_CYK.thy
@@ -2,6 +2,7 @@ theory Example_CYK
   imports Hnr_Diff_Arr Hnr_Array "HOL-Library.Code_Target_Nat" Definition_Utils
 begin
 
+(* TODO: Verify with original implementation from CYK.thy *)
 datatype ('n, 't) RHS = NonTerminals 'n 'n | Terminal 't 
 
 type_synonym ('n, 't) CNG = "('n \<times> ('n, 't) RHS) list"
@@ -10,6 +11,7 @@ fun member_original :: "'a \<Rightarrow> 'a list \<Rightarrow> bool" where
   "member_original a [] = False" 
 | "member_original a (x#xs) = (x = a \<or> member_original a xs)"
 
+(* TODO: Automatic rewriting to index-based iteration if tail is unused *)
 fun member :: "'a \<Rightarrow> 'a list \<Rightarrow> nat \<Rightarrow> bool" where
   "member a xs n = (case n of 
             0 \<Rightarrow> False 
@@ -33,77 +35,17 @@ definition member_opt where
       }
   )"
 
-method_setup partial_function_mono = \<open>Scan.succeed (SIMPLE_METHOD' o Partial_Function.mono_tac)\<close>
-
 schematic_goal member_opt_unfold: "member_opt a xs n \<equiv> ?v"
   apply(rule gen_code_thm_option_fixp[OF member_opt_def])
   by(partial_function_mono)
-  thm gen_code_thm_option_fixp option.mono_body_fixp
 
+thm gen_code_thm_option_fixp option.mono_body_fixp
 find_theorems "option.fixp_fun"
 
 lemma member_opt_termination: "member_opt a xs n = Some (member a xs n)"
   apply(induction a xs n rule: member.induct)
   apply(simp(no_asm) add: member.simps member_opt_unfold)
   by(auto split: nat.splits)
-
-lemma [simp]: "flat_lub b {} = b"
-  by (simp add: flat_lub_def)
-
-lemma [simp]: "fun_lub lub {} = (\<lambda>_. lub {})"
-  by (simp add: fun_lub_def)
-
-lemma admissible_fun:
-    fixes le:: "'a \<Rightarrow> 'a \<Rightarrow> bool" and Q :: "'b \<Rightarrow> 'a \<Rightarrow> bool"
-    assumes adm: "\<And>x. ccpo.admissible lub le (Q x)"
-    shows "ccpo.admissible  (fun_lub lub) (fun_ord le) (\<lambda>f. \<forall>x. Q x (f x))"
-  proof (rule ccpo.admissibleI)
-    fix A :: "('b \<Rightarrow> 'a) set"
-    assume Q: "\<forall>f\<in>A. \<forall>x. Q x (f x)"
-    assume ch: "Complete_Partial_Order.chain (fun_ord le) A"
-    assume "A \<noteq> {}"
-    hence non_empty: "\<And>a. {y. \<exists>f\<in>A. y = f a} \<noteq> {}" by auto
-    show "\<forall>x. Q x (fun_lub lub A x)"
-      unfolding fun_lub_def
-      by (rule allI, rule ccpo.admissibleD[OF adm chain_fun[OF ch] non_empty])
-        (auto simp: Q)
-  qed
-
-lemma admissible_flat: "ccpo.admissible (flat_lub b) (flat_ord b) (P)"
-  apply (rule ccpo.admissibleI)
-  by (metis all_not_in_conv flat_interpretation flat_lub_in_chain flat_ord_def partial_function_definitions.lub_upper)
-
-lemma hnr_recursion:
-  assumes 
-    mono_option: "\<And>x. mono_option (\<lambda>r. f r x)"
-  and
-    step: "\<And>r ri x xi. (\<And>x' xi'. hnr (\<Gamma> x' xi') (ri xi') (\<Gamma>' x' xi') (r x'))
-        \<Longrightarrow> hnr (\<Gamma> x xi) (fi ri xi) (\<Gamma>' x xi) (f r x)"
-  and
-    mono_heap: "\<And>x. mono_Heap (\<lambda>r. fi r x)"
-  shows  
-    "hnr (\<Gamma> x xi) (heap.fixp_fun fi xi) (\<Gamma>' x xi) (option.fixp_fun f x)"
-proof(induction arbitrary: x xi rule: ccpo.fixp_induct[OF option.ccpo])
-  case 1
-  then show ?case 
-    apply(rule admissible_fun)
-    by(rule admissible_flat)
-next
-  case 2
-  then show ?case 
-    using mono_option 
-    by(auto simp: monotone_def fun_ord_def)
-next
-  case 3
-  then show ?case 
-    by auto
-next
-  case 4
-  then show ?case 
-    apply(subst heap.mono_body_fixp[OF mono_heap])
-    apply(rule step)
-    by simp
-qed
  
 definition member_body where
   "member_body r a xs n =  (
@@ -150,30 +92,33 @@ function inner :: "('n, 't) CNG \<Rightarrow> (nat \<times> nat \<Rightarrow> 'n
   )"
 by pat_completeness auto
 termination
-by(relation "measure(\<lambda>(a, b, c, d, e). e - d)", rule wf_measure, simp)
+  by(relation "measure(\<lambda>(a, b, c, d, e). e - d)", rule wf_measure, simp)
+
+function main :: "('n, 't) CNG \<Rightarrow> (nat \<times> nat \<Rightarrow> 'n list) \<Rightarrow> nat \<Rightarrow> nat \<Rightarrow> nat \<Rightarrow> (nat \<times> nat \<Rightarrow> 'n list)"
+where "main G T len i j = (let T' = T((i, j) := inner G T i 1 j) in
+                            if i + j < len then main G T' len (i + 1) j
+                            else if j < len then main G T' len 0 (j + 1)
+                                 else T')"
+by pat_completeness auto
+termination 
+by(relation "inv_image (less_than <*lex*> less_than) (\<lambda>(a, b, c, d, e). (c - e, c - (d + e)))", rule wf_inv_image, rule wf_lex_prod, (rule wf_less_than)+, simp_all)
+
 
 context
   fixes x :: "'a :: heap"
   fixes xsi :: "'a cell ref"
 begin
 
-definition Ref where
-  "Ref A a b = A a b"
-
-schematic_goal "Ref id_assn a b \<Longrightarrow>\<^sub>A Ref ?A a (?b::?'b) * ?F" "undefined ?A ?b ?F"
-   apply(frame_inference_2_dbg \<open>rule ent_refl\<close>)
-  oops
-
 synth_definition member_impl is [hnr_rule_diff_arr]:
   "hnr (master_assn' (insert (xs, xsi) F) * id_assn n ni) (\<hole>:: ?'a Heap) ?\<Gamma>' (member_opt x xs n)"
   unfolding member_opt_def
   (* Could this problem partly be solved by the rule that the terminating branches always appear
-     first*)
+     first? *)
   supply r = hnr_recursion[where 
       \<Gamma> = "(\<lambda>n ni. master_assn' (insert (xs, xsi) F) * id_assn n ni)" and
       \<Gamma>' = "(\<lambda>n ni r ri. master_assn' (insert (xs, xsi) F) * id_assn n ni * id_assn r ri)"] 
   apply(rule r)
-  apply(partial_function_mono)
+  apply partial_function_mono
   apply hnr_diff_arr
   apply(rule hnr_fallback)
   apply(extract_pre rule: models_id_assn)
@@ -189,7 +134,7 @@ synth_definition member_impl is [hnr_rule_diff_arr]:
   apply(hypsubst)
   apply(rule refl)
   apply hnr_diff_arr
-  apply(partial_function_mono)
+  apply partial_function_mono
   done
 
 end
